{
 "cells": [
  {
   "cell_type": "markdown",
   "metadata": {},
   "source": [
    "# **11-Method of Undertermined Coefficients**\n",
    "\n",
    "---\n",
    "\n",
    "### **Introduction**\n",
    "\n",
    "This notebook goes over the method of undetermined coefficients for inhomogeneous problems.\n",
    "\n",
    "---\n",
    "\n",
    "### **Author**\n",
    "**Junichi Koganemaru**  \n",
    "\n",
    "---\n",
    "\n",
    "### **Last Updated**\n",
    "**February 1, 2025**"
   ]
  },
  {
   "cell_type": "markdown",
   "metadata": {},
   "source": [
    "# Method of undetermined coefficients\n",
    "\n",
    "Consider the inhomogeneous constant coefficient linear equation  \n",
    "$$\n",
    "a_n y^{(n)}(x) + a_{n-1} y^{(n-1)}(x) + \\cdots + a_1 y'(x) + a_0 y(x) = g(x), \\; x \\in I\n",
    "$$\n",
    "where $\\{a_i\\}_{i=1}^n$ are real-valued constants and $a_n \\neq 0$. \n",
    "Recall that the general solution to the equation is given by\n",
    "$$\n",
    "y(x) = y_p(x) + y_h(x), \\; x \\in I\n",
    "$$\n",
    "where the homogeneous solution $y_h$ is the general solution to the homogeneous equation, and a particular solution $y_p$ is any parameter free solution to the equation. \n",
    "\n",
    "We've learned that for constant coefficient linear equations, we can recover the homogeneous solution by examining the characteristic polynomial associated with the equation. To identify the general solution for the inhomogeneous problem, all that is left is to develop a mechanism to find a particular solution to the equation.\n",
    "\n",
    "Next, we'll go over the method of undetermined coefficients, which is a method for recovering a particular solution $y_p$ when $g$ is:\n",
    "1. a polynomial $P(\\cdot)$;\n",
    "2. an exponential $e^{\\alpha \\cdot}$;\n",
    "3. $\\sin(\\cdot)$ or $\\cos(\\cdot)$;\n",
    "4. any linear combination of products of (1), (2), (3).\n",
    "\n",
    "Note that the following functions do not fall into any of the categories above, which means that this method is not suitable for $g: I \\to \\mathbb{R}$ where:\n",
    "- $g(x) = \\ln x$ (not an exponential)\n",
    "- $g(x) = \\frac{1}{x}$ (not a polynomial) \n",
    "- $g(x) = \\tan(x), \\sin^{-1}(x)$ (not a linear combination of $\\sin$ and $\\cos$).\n",
    "\n",
    "## The main idea\n",
    "\n",
    "The main idea behind the method is to use an *ansatz* (a fancy German word for an educated guess): by exploiting the structure of $g$ and the ODE, we guess that $y_p$ takes a certain form with undetermined coefficients (constants to be determined). The task then reduces to finding the numerical value of these coefficients, and one can do so by substituting the ansatz into the ODE to get a system of equations for the coefficients. Let's consider a concrete example.\n",
    "\n",
    "> **Example**  \n",
    "> Consider the ODE  \n",
    "> $$  \n",
    "> y''(x) + 4y'(x) - 2y(x) = -2x^2 + 6x, \\; x \\in \\mathbb{R}\n",
    "> $$  \n",
    "> The homogeneous solution can be solved by looking at the roots of the characteristic polynomial. One can check that  \n",
    "> $$  \n",
    "> y_h(x) = c_1y_1(x) + c_2y_2(x) = c_1 e^{ (-2 - \\sqrt{6})x } + c_2 e^{ (-2 + \\sqrt{6})x }, \\; x \\in \\mathbb{R}\n",
    "> $$  \n",
    "> For a particular solution $y_p$, we guess that  \n",
    "> $$  \n",
    "> y_p = Ax^2 + Bx + C,  \n",
    "> $$  \n",
    "> where $A,B,C$ are constants to be determined. Then:  \n",
    "> $$  \n",
    "> \\begin{split}  \n",
    "> y_p' &= 2Ax + B\\\\  \n",
    "> y_p'' &= 2A.  \n",
    "> \\end{split}  \n",
    "> $$  \n",
    "> Substituting $y_p$ into the ODE gives us  \n",
    "> $$  \n",
    "> \\begin{split}  \n",
    "> y_p'' + 4y_p' - 2y_p &= 2A + 4(2Ax+B) - 2(Ax^2 + Bx +C) \\\\  \n",
    "> &= x^2(-2A) + x(8A - 2B) + (2A+4B - 2C) \\\\  \n",
    "> &=-2x^2 + 6x.  \n",
    "> \\end{split}  \n",
    "> $$  \n",
    "> Since the LHS and the RHS must be equal as polynomials, we must have  \n",
    "> $$  \n",
    "> \\begin{cases}  \n",
    "> -2A &= -2 \\\\  \n",
    "> 8A - 2B &= 6\\\\  \n",
    "> 2A + 4B - 2C &= 0  \n",
    "> \\end{cases} \\implies  \n",
    "> \\begin{cases}  \n",
    "> A &= 1 \\\\  \n",
    "> B &= 1 \\\\  \n",
    "> C &= 3.  \n",
    "> \\end{cases}  \n",
    "> $$  \n",
    "> Therefore a particular solution to the ODE is $y_p = x^2 + x + 3$. Therefore the general solution to the original equation is  \n",
    "> $$  \n",
    "> y(x) = y_p + y_h = x^2 + x + 3 + c_1 e^{ (-2 - \\sqrt{6})x } + c_2 e^{ (-2 + \\sqrt{6})x },  \\; x \\in \\mathbb{R}\n",
    "> $$  \n",
    "> where $c_1, c_2$ are arbitrary constants.  \n",
    "\n",
    "**Remark:** Note that a particular solution is not unique: we can always add a homogeneous solution to a particular solution and the function will still be a particular solution. For example,  \n",
    "$$  \n",
    "\\tilde{y}_p = x^2 + x + 3 + e^{(-2-\\sqrt{6})x}  \n",
    "$$  \n",
    "is also a parameter-free solution to the original equation, since  \n",
    "$$  \n",
    "L (\\tilde{y}_p) = L(y_p) + L( e^{(-2-\\sqrt{6})x} ) = -2x^2 + 6x + 0 = -2x^2 + 6x.  \n",
    "$$  \n",
    "So we can also write the general solution as  \n",
    "$$  \n",
    "y(x) = \\tilde{y}_p + y_h = (x^2 + x + 3 + e^{(-2-\\sqrt{6})x} ) + c_1 e^{ (-2 - \\sqrt{6})x } + c_2 e^{ (-2 + \\sqrt{6})x },  \\; x \\in \\mathbb{R}\n",
    "$$  \n",
    "where $c_1, c_2$ are arbitrary constants.  \n",
    "\n",
    "**Remark:** Note that in this example, our initial guess for $y_p$ doesn't contain any terms that are in $y_h$ (we call these duplicate terms). This turns out to be an important observation, and in general one should always work out $y_h$ first, as we'll need to modify our guess accordingly if our initial guess contains duplicate terms. We'll talk about this in the section to follow.  \n"
   ]
  },
  {
   "cell_type": "markdown",
   "metadata": {},
   "source": [
    "## Duplications in $y_p$ \n",
    "Consider the following example.\n",
    "\n",
    "> **Example**  \n",
    "> Consider the ODE  \n",
    "> $$  \n",
    "> y''(x) - y(x) = e^x, \\quad x \\in \\mathbb{R}.  \n",
    "> $$  \n",
    "> We start by solving for the homogeneous solution $y_h$. The characteristic polynomial is given by  \n",
    "> $$  \n",
    "> r^2 - 1 = 0 \\implies r_1 = 1, r_2 = -1.  \n",
    "> $$  \n",
    "> Therefore  \n",
    "> $$  \n",
    "> y_h(x) = c_1 e^x + c_2 e^{-x}.  \n",
    "> $$  \n",
    "> Since $g(x) = e^x$ our initial ansatz is  \n",
    "> $$  \n",
    "> y_p(x) = A e^x,  \n",
    "> $$  \n",
    "> but notice that $y_p$ is contained in $y_h$ ($c_1$ and $A$ are both arbitrary constants). This implies that $y_p$ in its current form is a homogeneous solution to the equation. In other words, $y_p''(x) - y_p(x)$ will be equal to 0 for all constants $A$, so $y_p$ cannot possibly be a particular solution to the inhomogeneous ODE.  \n",
    "> \n",
    "> The underlying issue is that we have duplicate terms in our ansatz $y_p$ and the homogeneous solution $y_h$, so we want to get rid of them by multiplying the initial ansatz by powers of $x$ ($x, x^2, x^3$, etc.). In this case we can eliminate the duplicate term by multiplying our initial ansatz by $x$. So the correct ansatz to use is  \n",
    "> $$  \n",
    "> y_p(x) = A x e^x.  \n",
    "> $$  \n",
    "> This gives us  \n",
    "> $$  \n",
    "> \\begin{split}  \n",
    "> y_p'(x) &= e^x( Ax + A) \\\\  \n",
    "> y_p''(x) &= e^x( Ax+ 2A).  \n",
    "> \\end{split}  \n",
    "> $$  \n",
    "> This implies that we should have  \n",
    "> $$  \n",
    "> y_p''(x) - y_p(x) = 2 A e^x = e^x \\implies A = \\frac{1}{2}.  \n",
    "> $$  \n",
    "> So a particular solution is given by  \n",
    "> $$  \n",
    "> y_p(x) = \\frac{1}{2} x e^x.  \n",
    "> $$  \n",
    "> This means that the general solution to the equation is  \n",
    "> $$  \n",
    "> y(x) = y_p(x) + y_h(x) = \\frac{1}{2} x e^x + c_1 e^x + c_2 e^{-x},  \n",
    "> $$  \n",
    "> where $c_1,c_2$ are arbitrary constants.  \n",
    "\n",
    "Let's do another example. \n",
    "\n",
    "> **Example**  \n",
    "> Consider the ODE  \n",
    "> $$  \n",
    "> y''(x) + 4y'(x) + 4y(x) = (x+3)e^{-2x}, \\quad x \\in \\mathbb{R}.  \n",
    "> $$  \n",
    "> We start by solving for the homogeneous solution $y_h(x)$. The characteristic polynomial is given by  \n",
    "> $$  \n",
    "> r^2 + 4r + 4 = 0 \\implies (r + 2)^2 = 0 \\implies r_1 = r_2 = -2.  \n",
    "> $$  \n",
    "> Therefore  \n",
    "> $$  \n",
    "> y_h(x) = c_1 e^{-2x} + c_2 x e^{-2x}.  \n",
    "> $$  \n",
    "> Since $g(x) = (x+3) e^{-2x}$, our (initial) ansatz is  \n",
    "> $$  \n",
    "> y_p(x) = (Ax+B) e^{-2x} = Ax e^{-2x} + B e^{-2x}.  \n",
    "> $$  \n",
    "> \n",
    "> Notice that in its current form $y_p$ is a linear combination of $e^{-2x}$ and $xe^{-2x}$ and so is $y_h$ (the previous equation is the same as the one before it just with different letters denoting the coefficients). This means that $y_p$ in its current form is a homogeneous solution. In other words, $y_p'' + 4y_p' + 4y_p$ is equal to the zero function for any constants $A$ and $B$, so $y_p$ cannot possibly be a particular solution to the original ODE.  \n",
    "> \n",
    "> The underlying issue is that we have duplicate terms in our ansatz $y_p$, so we look to get rid of them by multiplying the initial ansatz by powers of $x$ ($x, x^2, x^3$, etc.). In this case we see that to completely eliminate duplicate terms we should multiply our initial guess by $x^2$. Our second ansatz is  \n",
    "> $$  \n",
    "> y_p(x) = x^2 (Ax+B) e^{-2x} = (Ax^3 + Bx^2) e^{-2x}.  \n",
    "> $$  \n",
    "> Then  \n",
    "> $$  \n",
    "> \\begin{split}  \n",
    "> y_p'(x) &= ( -2(Ax^3 + Bx^2) + (3Ax^2 + 2Bx) ) e^{-2x} \\\\  \n",
    "> &= (-2Ax^3 + (3A - 2B)x^2 + 2Bx) e^{-2x} \\\\  \n",
    "> y_p''(x)&= ( -2(-2Ax^3 + (3A - 2B)x^2 + 2Bx) + (-6Ax^2 + 2(3A-2B)x + 2B) ) e^{-2x}\\\\  \n",
    "> &= ( 4Ax^3 + (-12A + 4B) x^2 + (6A - 8B)x + 2B) e^{-2x},  \n",
    "> \\end{split}  \n",
    "> $$  \n",
    "> and thus  \n",
    "> $$  \n",
    "> \\begin{split}  \n",
    "> y_p''(x) + 4y_p'(x) + 4y_p(x) &= e^{-2x} (4Ax^3 + (-12A + 4B) x^2 + (6A - 8B)x + 2B \\\\  \n",
    "> &\\quad \\quad \\quad+ 4(-2Ax^3 + (3A - 2B)x^2 + 2Bx) \\\\  \n",
    "> &\\quad \\quad \\quad+ 4( Ax^3 + Bx^2) )\\\\  \n",
    "> &= e^{-2x} ( 6A x + 2B).  \n",
    "> \\end{split}  \n",
    "> $$  \n",
    "> If $y_p''(x) + 4y_p'(x) + 4y_p(x) = (x+3)e^{-2x}$ then we require  \n",
    "> $$  \n",
    "> \\begin{cases}  \n",
    "> 6A &= 1 \\\\  \n",
    "> 2B & = 3  \n",
    "> \\end{cases} \\implies  \n",
    "> \\begin{cases}  \n",
    "> A &= \\frac{1}{6} \\\\  \n",
    "> B &= \\frac{3}{2}.  \n",
    "> \\end{cases}  \n",
    "> $$  \n",
    "> Therefore $y_p(x) = \\left( \\frac{1}{6} x^3 + \\frac{3}{2}x^2 \\right) e^{-2x}$ and the general solution is  \n",
    "> $$  \n",
    "> y(x) = y_h(x) + y_p(x) =  c_1 e^{-2x} + c_2 x e^{-2x} + \\left( \\frac{1}{6} x^3 + \\frac{3}{2}x^2 \\right) e^{-2x}.  \n",
    "> $$  \n",
    "\n",
    "**Remark**  \n",
    "Notice that when I took the derivatives of $y_p$ I always grouped the terms so that it's in the form of $e^{-2x} P(x)$. This is a good trick to keep in mind, as by grouping the terms this way you will only need to use the product rule once when you differentiate.\n"
   ]
  },
  {
   "cell_type": "markdown",
   "metadata": {},
   "source": [
    "## Linearity and table of ansatzes\n",
    "\n",
    "Below we list the common ansatzes associated to common types of inhomogeneous functions $f$ appearing on the right-hand side of a linear inhomogeneous differential equation. If one's initial guess overlaps with the general homogeneous solution of the equation, then we modify the guess by multiplying by a polynomial factor of $x^s$, where $s$ is the smallest non-negative integer such that no term in $y_p$ duplicates a term in the homogeneous solution. \n",
    "$$\n",
    "\\begin{array}{ | c | c |}\n",
    "     \\hline f & \\text{ansatz } y_p \\\\ \\hline\n",
    "     \\text{Polynomial } P_m(x) = a_0 + \\ldots + a_m x^m & \\text{Polynomial } \\textcolor{red}{x^s}(A_0 + \\ldots  + A_m x^m)  \\\\  \n",
    "     a \\cos k x + b \\sin k x \\text{ (one of } a \\text{ or } b \\text{ can be 0)} &  \\textcolor{red}{x^s}(A \\cos kx + B \\sin k x)\\\\  \n",
    "     e^{rx}(a \\cos k x + b \\sin k x) & \\textcolor{red}{x^s}e^{rx}(A \\cos kx + B \\sin k x) \\\\\n",
    "     P_m(x)e^{rx} & \\textcolor{red}{x^s}(A_0 + \\ldots  + A_m x^m)e^{rx}  \\\\\n",
    "     P_m(x)(a \\cos k x + b \\sin k x) & \\textcolor{red}{x^s}\\left[(A_0 + \\ldots  + A_m x^m)\\cos kx + (B_0 + \\ldots  + B_m x^m)\\sin kx \\right] \\\\\n",
    "     P_m(x)e^{rx}(a \\cos k x + b \\sin k x) & \\textcolor{red}{x^s}\\left[(A_0 + \\ldots  + A_m x^m)e^{rx}\\cos kx + (B_0 + \\ldots  + B_m x^m)e^{rx}\\sin kx \\right] \\\\\n",
    "     \\hline \n",
    "\\end{array}\n",
    "$$\n",
    "\n",
    "We note that if the equation is of the form \n",
    "$$\n",
    "     L(y(x)) = f_1(x) + f_2(x), \\quad x \\in \\mathbb{R},\n",
    "$$\n",
    "where $f_1, f_2$ are of two different types of functions appearing in the table above, then by taking advantage of the linearity of the equation, we can find two particular solutions $y_1, y_2$ satisfying \n",
    "$$\n",
    "     L(y_1(x)) = f_1(x), \\; L(y_2(x)) = f_2(x), \\quad x \\in \\mathbb{R},\n",
    "$$\n",
    "then $y_1 + y_2$ is a particular solution to the original equation:\n",
    "$$\n",
    "     L(y_1(x) + y_2(x)) = L(y_1(x)) + L(y_2(x)) = f_1(x) + f_2(x), \\quad x \\in \\mathbb{R}.\n",
    "$$\n",
    "Therefore for inhomogeneous functions of this type, when one applies the method of undetermined coefficients one would use an ansatz of the form \n",
    "$$\n",
    "     y_p(x) = y_{p,1}(x) + y_{p,2}(x), \\quad x \\in \\mathbb{R},\n",
    "$$\n",
    "where $y_{p,1}$ is the ansatz corresponding to $f_1$ and $y_{p,2}$ is the ansatz corresponding to $f_2$. If any modifications are needed due to duplications of the initial guess with the general homogeneous equations, the modifications are chosen *separately* for each ansatz appearing in the sum $y_p$."
   ]
  },
  {
   "cell_type": "markdown",
   "metadata": {},
   "source": [
    "## More examples\n",
    "\n",
    "> **Example**\n",
    "> Given that $y_{p_1}(x) = 3e^{2x}$ is a particular solution to \n",
    "> $$\n",
    "> y''(x) - 6y'(x) + 5y(x) = -9e^{2x}, \\quad x \\in \\mathbb{R}\n",
    "> $$\n",
    "> and that $y_{p_2}(x) = x^2 + 3x$ is a particular solution to \n",
    "> $$\n",
    "> y''(x) - 6y'(x) + 5y(x) = 5x^2 + 3x - 16, \\quad x \\in \\mathbb{R}\n",
    "> $$\n",
    "> suppose we want to find a particular solution to \n",
    "> $$\n",
    "> y''(x) - 6y'(x) + 5y(x) = -10x^2 - 6x + 32 + e^{2x}, \\quad x \\in \\mathbb{R}\n",
    "> $$\n",
    "> We first write the right hand side of the equation as a linear combination of $g_1(x)$ and $g_2(x)$. Notice that \n",
    "> $$\n",
    "> -10x^2 - 6x + 32 + e^{2x} = -2(5x^2 + 3x - 16) - \\frac{1}{9}(-9e^{2x}) = -2g_1(x) - \\frac{1}{9}g_2(x).\n",
    "> $$\n",
    "> Therefore, the equation can be written as \n",
    "> $$\n",
    "> y''(x) - 6y'(x) + 5y(x) = -2g_1(x) - \\frac{1}{9}g_2(x), \\quad x \\in \\mathbb{R}\n",
    "> $$ \n",
    "> and by linearity we get that \n",
    "> $$\n",
    "> y_p(x) = -2y_{p_2}(x) - \\frac{1}{9}y_{p_1}(x)\n",
    "> $$\n",
    "> is a particular solution to the equation.\n",
    "\n",
    "\n",
    "> **Example**\n",
    "> Suppose we want to solve the ODE \n",
    "> $$\n",
    "> y''(x) - 2y'(x) + 5y(x) = e^x \\cos(2x), \\quad x \\in \\mathbb{R}\n",
    "> $$\n",
    "> using the method of undetermined coefficients.\n",
    "> The characteristic polynomial associated with the ODE is \n",
    "> $$\n",
    "> r^2 - 2r + 5 = 0.\n",
    "> $$\n",
    "> The quadratic formula tells us that \n",
    "> $$\n",
    "> r = \\frac{2 \\pm \\sqrt{4 - 20}}{2} = 1 \\pm 2i,\n",
    "> $$\n",
    "> therefore the homogeneous solution is given by \n",
    "> $$\n",
    "> y_h(x) = c_1 e^x \\cos(2x) + c_2 e^x \\sin(2x).\n",
    "> $$\n",
    "> Notice that for $f(x) = e^x \\cos(2x)$, our guess should be \n",
    "> $$\n",
    "> y_p(x) = x (A\\cos(2x) + B\\sin(2x)) e^x = (Ax \\cos(2x) + Bx \\sin(2x))e^x\n",
    "> $$\n",
    "> to avoid duplications with the homogeneous solution. We calculate:\n",
    "> $$\n",
    "> \\begin{aligned}\n",
    "> y_p(x) &= (Ax \\cos(2x) + Bx \\sin(2x))e^x \\\\\n",
    "> y_p'(x) &= e^x( A( \\cos(2x) - 2x\\sin(2x)) + B( \\sin(2x) + 2x \\cos(2x)) + (Ax \\cos(2x) + Bx \\sin(2x))\\\\\n",
    "> &= e^x ( (A+2B) x\\cos(2x) + (B-2A) x\\sin(2x) + (A)\\cos(2x) + (B) \\sin(2x) ) \\\\\n",
    "> y_p''(x) &= e^x (  (A+2B)(\\cos(2x) - 2x\\sin(2x)) + (B-2A) ( \\sin(2x) + 2x \\cos(2x)) - 2A \\sin(2x) + 2B \\cos(2x) \\\\\n",
    "> &\\quad + (A+2B) x\\cos(2x) + (B-2A) x\\sin(2x) + (A)\\cos(2x) + (B) \\sin(2x) )\\\\\n",
    "> &= e^x ( (4B - 3A) x\\cos(2x) + (-4A - 3B) x\\sin(2x) + (2A+4B) \\cos(2x) + (2B-4A) \\sin(2x))\\\\\n",
    "> y_p''(x) - 2y_p'(x) + 5y_p(x) &= \\\\\n",
    "> &e^x ( a x\\cos(2x) + bx\\sin(2x) + c \\cos(2x) + d\\sin(2x)) \\\\\n",
    "> &= e^x \\cos(2x)\n",
    "> \\end{aligned}\n",
    "> $$\n",
    "> with \n",
    "> $$\n",
    "> \\begin{aligned}\n",
    "> a &=(4B-3A) - 2(A+2B) + 5(A) = 0 \\\\\n",
    "> b&= (-4A - 3B) - 2( B-2A) + 5(B) = 0 \\\\\n",
    "> c&= (2A+4B) - 2(A) + 5(0) = 4B\\\\\n",
    "> d&= (2B-4A) -2(B)  +5(0) = -4A.\n",
    "> \\end{aligned}\n",
    "> $$\n",
    "> We should have $a=b=d=0, c=1$, therefore $4B = 1 \\implies B = 1/4$ and $-4A = 0 \\implies A =0$. So\n",
    "> $$\n",
    "> y_p(x) = \\left( \\frac{1}{4} x \\sin(2x) \\right)e^x.\n",
    "> $$\n",
    "> The general solution is then given by \n",
    "> $$\n",
    "> y(x) = y_h(x) + y_p(x) = c_1 e^x \\cos(2x) + c_2 e^x \\sin(2x) +\\left( \\frac{1}{4} x \\sin(2x) \\right) e^x.\n",
    "> $$\n",
    "\n",
    "\n",
    "> **Example**\n",
    "> Suppose we want to solve the given ODE \n",
    "> $$\n",
    "> \\begin{cases}\n",
    "> y''(x) - 4y'(x) + 4y(x) = (12x^2 - 6x) e^{2x}, \\quad x \\in \\mathbb{R}\\\\\n",
    "> y(0) = 1\\\\\n",
    "> y'(0) = 0.\n",
    "> \\end{cases}\n",
    "> $$\n",
    "> using the method of undetermined coefficients.\n",
    "> \n",
    "> The characteristic polynomial is given by \n",
    "> $$\n",
    "> r^2 - 4r + 4 = 0 \\implies (r-2)^2 = 0 \\implies r_1 = 2, r_2 = 2.\n",
    "> $$\n",
    "> The homogeneous solution is then given by \n",
    "> $$\n",
    "> y_h(x)= c_1 e^{2x} + c_2 x e^{2x}.\n",
    "> $$\n",
    "> Our guess for a particular solution should be \n",
    "> $$\n",
    "> \\begin{aligned}\n",
    "> y_p(x) &= x^2 (Ax^2 + Bx + C) e^{2x}\\\\\n",
    "> &= (Ax^4 + Bx^3 + Cx^2 ) e^{2x}\n",
    "> \\end{aligned}\n",
    "> $$\n",
    "> to avoid duplications with the homogeneous solution. Now we calculate:\n",
    "> $$\n",
    "> \\begin{aligned}\n",
    "> y_p(x) &=   e^{2x}(Ax^4 + Bx^3 + Cx^2)\\\\\n",
    "> y_p'(x) &= e^{2x} ( 4Ax^3 + 3Bx^2 + 2Cx + 2(Ax^4 + Bx^3 + Cx^2) )\\\\\n",
    "> &= e^{2x} ( 2Ax^4 + (4A+2B)x^3 + (3B + 2C)x^2 + 2Cx)\\\\\n",
    "> y_p''(x) &= e^{2x} (  8Ax^3 + 3(4A+2B)x^2 + 2(3B+2C)x + 2C + 2( 2Ax^4 + (4A+2B)x^3 + (3B + 2C)x^2 + 2Cx) ) \\\\\n",
    "> &= e^{2x} ( 4Ax^4 + (16A + 4B) x^3 + (12A + 12B + 4C) x^2 + (6B+8C)x + 2C ).\n",
    "> \\end{aligned}\n",
    "> $$\n",
    "> Then\n",
    "> $$\n",
    "> \\begin{aligned}\n",
    "> y_p''(x) - 4y_p'(x) + 4y_p(x) = e^{2x} (  ax^4 + bx^3 + cx^2 + dx + e) = e^{2x}(12x^2 - 6x), \\quad x \\in \\mathbb{R}\n",
    "> \\end{aligned} \n",
    "> $$\n",
    "> for \n",
    "> $$\n",
    "> \\begin{aligned}\n",
    "> a&=(4A) - 4(2A) + 4(A) = 0\\\\\n",
    "> b&=(16A+4B) - 4(4A+2B) + 4(B) = 0\\\\\n",
    "> c&=(12A+12B+4C) - 4(3B+2C) + 4(C) = 12A \\\\\n",
    "> d&=(6B + 8C) - 4(2C) + 4(0) = 6B\\\\\n",
    "> e&=2C  \n",
    "> \\end{aligned} \n",
    "> $$\n",
    "> Therefore we should have\n",
    "> $$\n",
    "> \\begin{aligned}\n",
    "> c &= 12A = 12 \\implies A = 1\\\\\n",
    "> d &= 6B = - 6 \\implies B = -1 \\\\\n",
    "> e &= 2C = 0 \\implies C = 0.\n",
    "> \\end{aligned}\n",
    "> $$\n",
    "> So a particular solution is given by\n",
    "> $$\n",
    "> y_p(x) = (x^4 - x^3)e^{2x}\n",
    "> $$\n",
    "> and the general solution to the ODE is then given by \n",
    "> $$\n",
    "> y(x) = c_1e^{2x} + c_2x e^{2x} + (x^4 - x^3)e^{2x}.\n",
    "> $$\n",
    "> This implies that $y'(x) = 2c_1 e^{2x} + e^{2x}( c_2 + 2c_2x) + e^{2x}( 4x^3 - 3x^2 +2(x^4 - x^3))$. Using the initial conditions we obtain $c_1 = 1$ and $c_2 = -2$."
   ]
  }
 ],
 "metadata": {
  "language_info": {
   "name": "python"
  }
 },
 "nbformat": 4,
 "nbformat_minor": 2
}
